Add example of relational properties proof with use of relational properties

Examples.v
@@ -66,16 +66,16 @@ Ltac mem_s s l1 l2 v :=
        rewrite Heax by lia;
        clear Heax.
 
+Ltac mem_s_in s l1 l2 v :=
+       generalize (set'def s l1 v l2);
+       intros Heax; destruct Heax as ( Heax & _);
+       rewrite Heax; clear Heax.
+
 Ltac mem_d s l1 l2 v :=
        generalize (set'def s l1 v l2);
        intros Heax; destruct Heax as ( _ & Heax);
        rewrite Heax; [ | first [ lia | (intros HF; inversion HF)]];
        clear Heax.
-
-Ltac mem_s_in s l1 l2 v :=
-       generalize (set'def s l1 v l2);
-       intros Heax; destruct Heax as ( Heax & _);
-       rewrite Heax; clear Heax.
 
 Ltac mem_d_in s l1 l2 v:=
        generalize (set'def s l1 v l2);
@@ -86,7 +86,7 @@ Ltac mem_d_in s l1 l2 v:=
 
 Parameter f : Proc.t.
 
-(* Body of procedure f: perfom multiplication *)
+(* Body of procedure f (multiplication) *)
 
 Definition mult: com := <[
   if 0 <= X1 && ~ X1 = 0 then
@@ -105,11 +105,11 @@ Definition f_psi (x': Proc.t) :=
 (* Contract of pre and post condition of procedure f *)
 
 Definition f_pre: precondition := fun s =>
-   s(X2) = (s(X3)) * (s(X4) - s(X1)) /\
-   0 <= (s(X1)) /\ Nat.le (s(X1)) (s(X4)).
+   s(X2) = s(X3) * (s(X4) - s(X1)) /\
+   0 <= s(X1) /\ Nat.le (s(X1)) (s(X4)).
 
-Definition f_post: postcondition := fun s _ =>
-  s(X2) = (s(X3)) * (s(X4)).
+Definition f_post: postcondition := fun s s' =>
+  s(X2) = s'(X3) * s'(X4).
 
 (* Contract environment *)
 
@@ -118,22 +118,24 @@ Definition f_phi (x': Proc.t) :=
 
 (* Program computing the multiplication of X3 and X4 and put the result in X2 *)
 
-Definition com_1 := <[
+Definition com_mult := <[
   X1 := X4;
   X2 := 0;
   call(f)
 ]>.
 
-Example hoare_triple_mult: hoare_triple (fun _ => True) f_post com_1 f_psi.
+(* Proof that command com_mult satisfies the 
+   postcondition f_post ( X2 = X3 * X4) *)
+Example hoare_triple_mult: hoare_triple (fun _ => True) f_post com_mult f_psi.
 Proof.
 apply correct with (cl:=f_phi) (l:=[]).
-(* Verification of proof obligation for procedure*)
+(* Verification of proof obligation for procedures *)
 * unfold f_psi, f_phi.
   apply Vcg_Opt.tc_p_same.
   intros f0.
   destruct (Proc.eqb f0 f) eqn: E.
   + split.
-     (* Verification of auxilliary proof obligation for procedure f*)
+     (* Verification of auxilliary proof obligation for procedure f *)
     - apply Vcg_Opt.Tc'_list.tc'_list_same.
       simpl.
       destruct n.
@@ -155,12 +157,10 @@ apply correct with (cl:=f_phi) (l:=[]).
          mem_d m X2 X1 (m X2 + m X3).
          simpl in H.
          unfold f_pre in H.
-         split.
-         ++ destruct H.
-            replace ((m X4 - (m X1 - 1))) with (S (m X4 - m X1 )).
-            rewrite Loc.mul_succ_r.
-            all : try lia.
-         ++ split. all: try lia.
+         destruct H.
+         replace ((m X4 - (m X1 - 1))) with (S (m X4 - m X1 )) by lia.
+         rewrite Loc.mul_succ_r.
+         lia.
       ** destruct n; [auto | auto].
     (* Main proof obligation for procedure f : the postconditon hold*)
     - simpl.
@@ -168,7 +168,17 @@ apply correct with (cl:=f_phi) (l:=[]).
       destruct H0.
       ** decompose [and] H1;clear H1.
          rewrite Proc.eqb_refl in H6.
-         apply H6.
+         simpl in H6.
+         unfold f_post in H6.
+         unfold f_post.
+         rewrite  H6.
+         rewrite H4.
+         mem_d m'' X1 X3 (m'' X1 - 1).
+         mem_d m'' X1 X4 (m'' X1 - 1).
+         rewrite H2.
+         mem_d m X2 X3 (m X2 + m X3).
+         mem_d m X2 X4 (m X2 + m X3).
+         reflexivity.
       ** rewrite H1.
          unfold f_post.
          simpl in H.
@@ -205,7 +215,16 @@ apply correct with (cl:=f_phi) (l:=[]).
     simpl.  intros.
     rewrite Proc.eqb_refl in H3.
     simpl in H3.
-    apply H3.
+    unfold f_post in H3.
+    unfold f_post.
+    rewrite H3.
+    rewrite H1.
+    mem_d m' X2 X3 0.
+    mem_d m' X2 X4 0.
+    rewrite H0.
+    mem_d m X1 X3 (m X4).
+    mem_d m X1 X4 (m X4).
+    reflexivity.
 Qed.
 
 (** Some ltac to automatize the extraction of proof obligation from the list construct
@@ -276,7 +295,7 @@ Ltac ltc0 phi l hyh := apply rcorrect
 (** Examples of proofs of Relational Properties
     with verification condition generator **)
 
-(* Example 1 *)
+(** Example 1: Swap **)
 
 (* Defintion of a swap functions *)
 
@@ -294,7 +313,7 @@ Definition swap_2: com := <[ °X1 := °X1 + °X2;
 
 Definition rela_pre : r_precondition := fun l =>
   match l with
-  | (m1 :: m2 :: []) => m1 (m1 X1) = m2 (m2 X1) /\ m1 (m1 X2) = m2 (m2 X2) /\
+  | [m1; m2] => m1 (m1 X1) = m2 (m2 X1) /\ m1 (m1 X2) = m2 (m2 X2) /\
                          m1 X1 > 3 /\ m1 X2 > 3 /\ m2 X1 > 3 /\ m2 X2 > 3 /\
                          m1 X1 <> m1 X2 /\ m2 X1 <> m2 X2
   | _ => False
@@ -302,18 +321,18 @@ Definition rela_pre : r_precondition := fun l =>
 
 Definition rela_post : r_postcondition := fun l _ =>
   match l with
-  | (m1 :: m2 :: []) => m1 (m1 X1) = m2 (m2 X1) /\ m1 (m1 X2) = m2 (m2 X2)
+  | [m1; m2] => m1 (m1 X1) = m2 (m2 X1) /\ m1 (m1 X2) = m2 (m2 X2)
   | _ => False
   end.
 
 Example relation_swap : relational_prop
                             rela_pre rela_post
-                            (swap_1 :: swap_2 :: []) Psi.empty_psi.
+                            [swap_1; swap_2] Psi.empty_psi.
 Proof.
-assert (hyh :length (swap_1 :: swap_2 :: []) = 
-             length (empty_history:: empty_history :: [])).
+assert (hyh :length [swap_1; swap_2] = 
+             length [empty_history; empty_history]).
 {  simpl. reflexivity. }
-ltc0 R_Phi.empty_r_phi (empty_history :: empty_history :: []) hyh.
+ltc0 R_Phi.empty_r_phi [empty_history; empty_history] hyh.
 (* Verification of proof obligation for procedure*)
 + apply rtc_p_empty_psi.
 (* Verification of auxilliary proof obligation *)
@@ -454,41 +473,44 @@ ltc0 R_Phi.empty_r_phi (empty_history :: empty_history :: []) hyh.
       lia.
 Qed.
 
-(* Example 2 *)
+(** Example 2: Compare **)
 
 (* Defintion of a comparator function *)
 
-Definition comp: com := <[ if X1 <= X2 && ~ X1 = X2 then
-                                 ret := 0
-                              else
-                                 if X2 <= X1 && ~ X1 = X2  then
-                                   ret := 2
-                                 else ret := 1
-                                 end
-                              end ]>.
+Definition comp: com := 
+<[ if X1 <= X2 && ~ X1 = X2 then
+      ret := 0
+   else
+      if X2 <= X1 && ~ X1 = X2  then
+         ret := 2
+      else 
+         ret := 1
+      end
+   end 
+]>.
 
 (* Defintion of relational pre and post condition *)
 
 Definition rela_pre_comp : r_precondition := fun l =>
   match l with
-  | (m1 :: m2 :: []) => m1 X1 = m2 X2 /\ m1 X2 = m2 X1
+  | [m1; m2] => m1 X1 = m2 X2 /\ m1 X2 = m2 X1
   | _ => False
   end.
 
 Definition rela_post_comp : r_postcondition := fun l _ =>
   match l with
-  | (m1 :: m2 :: []) => m1 ret + (m2 ret) = 2
+  | [m1; m2] => m1 ret + (m2 ret) = 2
   | _ => False
   end.
 
 Example relation_comp : relational_prop
                             rela_pre_comp rela_post_comp
-                            (comp :: comp :: []) Psi.empty_psi.
+                            [comp; comp] Psi.empty_psi.
 Proof.
-assert (hyh :length (comp :: comp :: []) = 
-             length (empty_history:: empty_history :: [])).
+assert (hyh :length [comp; comp] = 
+             length [empty_history; empty_history]).
 {  simpl. reflexivity. }
-ltc0 R_Phi.empty_r_phi (empty_history :: empty_history :: []) hyh.
+ltc0 R_Phi.empty_r_phi [empty_history; empty_history] hyh.
 (* Verification of proof obligation for procedure*)
 + apply rtc_p_empty_psi.
 (* Verification of auxilliary proof obligation *)
@@ -523,7 +545,7 @@ ltc0 R_Phi.empty_r_phi (empty_history :: empty_history :: []) hyh.
                reflexivity.
 Qed.
 
-(* Example 3 *)
+(** Example 3: Monotone **)
 
 (** Examples of proofs of relational properties using relational contract **)
 
@@ -538,13 +560,13 @@ Definition f2_psi (x': Proc.t) :=
 
 Definition f2_r_pre : r_precondition := fun l =>
   match l with
-  | (m1 :: m2 :: []) => m1 X1 < m2 X1
+  | [m1; m2] => m1 X1 < m2 X1
   | _ => False
   end.
 
 Definition f2_r_post : r_postcondition := fun l _ =>
   match l with
-  | (m1 :: m2 :: []) => m1 X1 < m2 X1
+  | [m1; m2] => m1 X1 < m2 X1
   | _ => False
   end.
 
@@ -552,13 +574,13 @@ Definition f2_r_post : r_postcondition := fun l _ =>
 
 Definition f2_pre : r_precondition := fun l =>
   match l with
-  | (m :: []) => True
+  | [m] => True
   | _ => False
   end.
 
 Definition f2_post : r_postcondition := fun l _ =>
   match l with
-  | (m1 :: []) => True
+  | [m1] => True
   | _ => False
   end.
 
@@ -567,23 +589,23 @@ Definition f2_post : r_postcondition := fun l _ =>
 Scheme Equality for list.
 
 Definition f2_r_phi (x': list Proc.t) :=
-        if (list_beq  Proc.t) Proc.eqb x' (f2 :: f2 :: []) 
+        if (list_beq  Proc.t) Proc.eqb x' [f2; f2]
         then (f2_r_pre,f2_r_post) 
         else
-            if (list_beq  Proc.t) Proc.eqb x' (f2 :: []) 
+            if (list_beq  Proc.t) Proc.eqb x' [f2]
             then (f2_pre,f2_post) 
             else R_Phi.empty_r_phi x'.
 
-(** Relation Propery **)
+(* Relation Propery *)
 
 Example relation_mono : relational_prop
                   f2_r_pre f2_r_post
-                  (<[ call(f2) ]> :: <[ call(f2) ]> :: []) f2_psi.
+                  [<[ call(f2) ]>; <[ call(f2) ]> ] f2_psi.
 Proof.
-assert (hyh :length (<[ call(f2) ]>:: <[ call(f2) ]> :: []) = 
-             length (empty_history:: empty_history :: [])).
+assert (hyh :length [<[ call(f2) ]>; <[ call(f2) ]>] = 
+             length [empty_history; empty_history]).
 {  simpl. reflexivity. }
-ltc0 f2_r_phi (empty_history :: empty_history :: []) hyh.
+ltc0 f2_r_phi [empty_history; empty_history] hyh.
 (* Verification of proof obligation for procedure *)
 + unfold rtc_p.
   intros.
@@ -618,8 +640,8 @@ ltc0 f2_r_phi (empty_history :: empty_history :: []) hyh.
          rewrite Proc.eqb_refl in H.
          simpl in H.
          assumption.
-   (* Verification of proof obligation for procedure f2*)
     - destruct (list_beq Proc.t Proc.eqb f0 [f2]) eqn: E2.
+       (* Verification of proof obligation for procedure f2*)
         * apply internal_list_dec_bl in E2 ;[ | apply Proc.eqb_eq ].
           subst.
           destruct m;[ discriminate hy1 | ].
@@ -639,6 +661,7 @@ ltc0 f2_r_phi (empty_history :: empty_history :: []) hyh.
              simpl.
              intros.
              auto.
+         (* Nothing to do for other procedure *)
          * unfold f2_r_phi in H.
            rewrite E1 in H.
            rewrite E2 in H.
@@ -662,35 +685,28 @@ ltc0 f2_r_phi (empty_history :: empty_history :: []) hyh.
 (* Main proof obligation *)
 + simpl.
   intros.
-  specialize (Hr (f2 :: f2 :: [])).
+  specialize (Hr [f2; f2]).
   unfold f2_r_phi in Hr.
-  replace (list_beq Proc.t Proc.eqb [f2; f2] [f2; f2]) with true in Hr.
-  - specialize (Hr (s :: s0 :: []) (m' :: m'0 :: [])).
+  rewrite internal_list_dec_lb in Hr; [ | apply Proc.eqb_eq | reflexivity].
+  - specialize (Hr [s; s0 ] [m'; m'0]).
     simpl in Hr.
     apply Hr.
-    all: try Lia.lia.
+    all: try lia.
     split. apply H0.
     split. apply H1.
     auto.
-  - simpl.
-    symmetry.
-    eapply Bool.andb_true_iff.
-    split.
-    apply Proc.eqb_eq. reflexivity.
-    eapply Bool.andb_true_iff.
-    split.
-    apply Proc.eqb_eq. reflexivity.
-    auto.
  Qed.
 
-(* Example 4 *)
+(** Example 4: Mult **)
+
+(** Examples of proofs of relational properties using relational contract **)
 
 (* Defintion of a sum functions *)
 
 Parameter f3 : Proc.t.
 
 Definition f3_body: com := <[
-  if X1 <= X2 && ~ X1 = 0 then
+  if X1 <= X2 && ~ X1 = X2 then
       X3 := X3 + X1;
       X1 := X1 + 1;
       call(f3)
@@ -707,15 +723,16 @@ Definition f3_psi (x': Proc.t) :=
 
 Definition f3_r_pre : r_precondition := fun l =>
   match l with
-  | (m1 :: m2 :: []) => m1 X2 = m2 X2 /\
+  | [m1; m2] => m2 X1 <= m2 X2 /\ ~ (m2 X1 = m2 X2) /\
+                        m1 X2 = m2 X2 /\
                         m1 X1 = m2 X1 + 1 /\
-                        m1 X3 = m2 X3 + m1 X1
+                        m1 X3 = m2 X3 + m2 X1
   | _ => False
   end.
 
 Definition f3_r_post : r_postcondition := fun l _ =>
   match l with
-  | (m1 :: m2 :: []) => m1 X3 = m2 X3
+  | [m1; m2] => m1 X3 = m2 X3
   | _ => False
   end.
 
@@ -723,54 +740,52 @@ Definition f3_r_post : r_postcondition := fun l _ =>
 
 Definition f3_pre : r_precondition := fun l =>
   match l with
-  | (m :: []) => True
+  | [m] => True
   | _ => False
   end.
 
-Definition f3_post : r_postcondition := fun l _ =>
-  match l with
-  | (m1 :: []) => True
-  | _ => False
+Definition f3_post : r_postcondition := fun l_pre l_post =>
+  match l_pre, l_post with
+  | [m_post],[m_pre] => m_pre X1 >= m_pre X2 -> m_pre X3 = m_post X3
+  | _,_ => False
   end.
 
 (* Definition of relational pre and post condition *)
 
 Definition r_pre : r_precondition := fun l =>
   match l with
-  | (m1 :: m2 :: []) => m1 X2 = m2 X2 /\
-                        m1 X1 = 0 /\ m2 X1 = 1 /\
-                        m1 X3 = 0 /\ m2 X3 = 0
+  | [m1; m2] => m1 X2 = m2 X2
   | _ => False
   end.
 
 Definition r_post : r_postcondition := fun l _ =>
   match l with
-  | (m1 :: m2 :: []) => m1 X3 = m2 X3
+  | [m1; m2] => m1 X3 = m2 X3
   | _ => False
   end.
 
 (* Relational contract environment *)
 
 Definition f3_r_phi (x': list Proc.t) :=
-        if (list_beq  Proc.t) Proc.eqb x' (f3 :: f3 :: []) 
+        if (list_beq  Proc.t) Proc.eqb x' [f3;f3] 
         then (f3_r_pre,f3_r_post) 
         else
-            if (list_beq  Proc.t) Proc.eqb x' (f3 :: []) 
-            then (f2_pre,f2_post) 
+            if (list_beq  Proc.t) Proc.eqb x' [f3]
+            then (f3_pre,f3_post) 
             else R_Phi.empty_r_phi x'.
 
 (** Relation Propery **)
 
 Example relation_sum : relational_prop
                   r_pre r_post
-                  (<[ X1:= 0; X3 := 0; call(f3) ]> :: 
-                   <[ X1:= 1; X3 := 0; call(f3) ]> :: []) f3_psi.
+                  [<[ X1:= 1; X3 := 0; call(f3) ]>;
+                   <[ X1:= 0; X3 := 0; call(f3) ]> ] f3_psi.
 Proof.
-assert (hyh :length  (<[ X1:= 0; X3 := 0; call(f3) ]> :: 
-                   <[ X1:= 1; X3 := 0; call(f3) ]> :: []) = 
-             length (empty_history:: empty_history :: [])).
+assert (hyh :length  [<[ X1:= 1; X3 := 0; call(f3) ]>;
+                      <[ X1:= 0; X3 := 0; call(f3) ]> ] = 
+             length [empty_history; empty_history]).
 {  simpl. reflexivity. }
-ltc0 f3_r_phi (empty_history :: empty_history :: []) hyh.
+ltc0 f3_r_phi [empty_history; empty_history] hyh.
 (* Verification of proof obligation for procedure *)
 + unfold rtc_p.
   intros.
@@ -799,7 +814,7 @@ ltc0 f3_r_phi (empty_history :: empty_history :: []) hyh.
                rewrite Proc.eqb_refl.
                simpl.
                auto.
-            **  destruct n; [auto | auto].
+           **  destruct n; [auto | auto].
          ++ split; [ | auto].
             apply Vcg_Opt.tc'_same.
             apply Vcg_Opt.Tc'_list.tc'_list_same.
@@ -813,7 +828,7 @@ ltc0 f3_r_phi (empty_history :: empty_history :: []) hyh.
                rewrite Proc.eqb_refl.
                simpl.
                auto.
-            **  destruct n; [auto | auto].
+           **  destruct n; [auto | auto].
        (* Main proof obligation *)
        * ltc5 f3_r_phi ps' hy1 hy2.
          unfold f3_psi, f3_r_phi.
@@ -825,55 +840,69 @@ ltc0 f3_r_phi (empty_history :: empty_history :: []) hyh.
          intros.
          destruct H2.
          ++ destruct H1.
-          ** specialize (H0 (f3 :: f3 :: [])).
+          ** specialize (H0 [f3; f3] [m''0;m''2] [m'; m'0]).
+             simpl in H0.
              unfold f3_r_phi in H0.
-             replace (list_beq Proc.t Proc.eqb [f3; f3] [f3; f3]) with true in H0.
-             specialize (H0 (m''0 :: m''2 :: []) (m' :: m'0 :: [])).
+             rewrite internal_list_dec_lb in H0; [ | apply Proc.eqb_eq | reflexivity].
              simpl in H0.
              apply H0; clear H0.
-             all: try Lia.lia.
+             all: try lia.
              split. apply H4.
              split. apply H3.
              auto.
              decompose [and] H3;clear H3.
              decompose [and] H4;clear H4.
              rewrite H10.
-             mem_d_in m'' X1 X2 (m'' X1 + 1).
-             mem_d_in m'' X1 X3 (m'' X1 + 1).
+             mem_d m'' X1 X2 (m'' X1 + 1).
+             mem_d m'' X1 X3 (m'' X1 + 1).
              mem_s m'' X1 X1 (m'' X1 + 1).
              rewrite H3.
-             mem_d_in s X3 X2 (s X3 + s X1).
-             mem_d_in s X3 X1 (s X3 + s X1).
+             mem_d s X3 X2 (s X3 + s X1).
+             mem_d s X3 X1 (s X3 + s X1).
              mem_s s X3 X3 (s X3 + s X1).
              rewrite H6.
-             mem_d_in m''1 X1 X2 (m''1 X1 + 1).
-             mem_d_in m''1 X1 X3 (m''1 X1 + 1).
+             mem_d m''1 X1 X2 (m''1 X1 + 1).
+             mem_d m''1 X1 X3 (m''1 X1 + 1).
              mem_s m''1 X1 X1 (m''1 X1 + 1).
              rewrite H0.
-             mem_d_in s0 X3 X2 (s0 X3 + s0 X1).
-             mem_d_in s0 X3 X1 (s0 X3 + s0 X1).
+             mem_d s0 X3 X2 (s0 X3 + s0 X1).
+             mem_d s0 X3 X1 (s0 X3 + s0 X1).
              mem_s s0 X3 X3 (s0 X3 + s0 X1).
              unfold f3_r_phi in H.
-             replace (list_beq Proc.t Proc.eqb [f3; f3] [f3; f3]) with true in H.
+             rewrite internal_list_dec_lb in H; [ | apply Proc.eqb_eq | reflexivity].
              simpl in H.
-             Lia.lia.
-             simpl.
-             rewrite Proc.eqb_refl.
-             auto.
-             all: unfold X1, X2, X3.
-             all: try Lia.lia.
-             simpl.
-             rewrite Proc.eqb_refl.
-             auto.
-          **
-             
-         
-         
-         
-         
-         
-   (* Verification of proof obligation for procedure f2*)
-    - destruct (list_beq Proc.t Proc.eqb f0 [f2]) eqn: E2.
+             lia.
+          ** decompose [and] H3;clear H3.
+             unfold f3_r_phi in H.
+             rewrite internal_list_dec_lb in H; [ | apply Proc.eqb_eq | reflexivity].
+             simpl in H.
+             destruct H.
+             destruct H3.
+             rewrite H4.
+             rewrite <- H8.
+             rewrite H7.
+             mem_d m''1 X1 X3 (m''1 X1 + 1).
+             rewrite H5.
+             mem_s s0 X3 X3 (s0 X3 + s0 X1).
+             lia.
+             rewrite H7.
+             mem_s m''1 X1 X1 (m''1 X1 + 1).
+             mem_d m''1 X1 X2 (m''1 X1 + 1).
+             rewrite H5.
+             mem_d s0 X3 X1 (s0 X3 + s0 X1).
+             mem_d s0 X3 X2 (s0 X3 + s0 X1).
+             lia.
+         ++ destruct H1.
+          ** unfold f3_r_phi in H.
+             rewrite internal_list_dec_lb in H; [ | apply Proc.eqb_eq | reflexivity].
+             simpl in H.
+             lia.
+          ** unfold f3_r_phi in H.
+             rewrite internal_list_dec_lb in H; [ | apply Proc.eqb_eq | reflexivity].
+             simpl in H.
+             lia.
+    - destruct (list_beq Proc.t Proc.eqb f0 [f3]) eqn: E2.
+       (* Verification of proof obligation for procedure f3*)
         * apply internal_list_dec_bl in E2 ;[ | apply Proc.eqb_eq ].
           subst.
           destruct m;[ discriminate hy1 | ].
@@ -881,58 +910,126 @@ ltc0 f3_r_phi (empty_history :: empty_history :: []) hyh.
           split.
           (* Verification of auxilliary proof obligation *)
           ** simpl.
-             unfold f2_psi.
+             unfold f3_psi.
              rewrite Proc.eqb_refl.
+             split; [ | auto].
+             apply Vcg_Opt.tc'_same.
+             apply Vcg_Opt.Tc'_list.tc'_list_same.
              simpl.
-             auto.
+             destruct n.
+             ++ unfold Vcg_Opt.Tc'_list.continuation.
+                simpl.
+                intros.
+                unfold f3_r_phi.
+                simpl.
+                rewrite Proc.eqb_refl.
+                simpl.
+                auto.
+             ++ destruct n; [auto | auto].
           (* Main proof obligation *)
-          ** simpl.
-             unfold f2_psi, f2_r_phi.
+          ** ltc5 f3_r_phi ps' hy1 hy2.
+             unfold f3_psi, f3_r_phi.
+             simpl.
+             rewrite Proc.eqb_refl.
              simpl.
              rewrite Proc.eqb_refl.
              simpl.
              intros.
-             auto.
-         * unfold f2_r_phi in H.
-           rewrite E1 in H.
-           rewrite E2 in H.
-           simpl in H.
-           unfold empty_r_precondition in H.
-           contradiction.
-(* Proof obligation for relational property 
-      {f2_r_pre} <[ call(f2) ]> ~ <[ call(f2) ]> {f2_r_post} 
-*)
+             destruct H1.
+             ++ lia.
+             ++ rewrite H3.
+                reflexivity.
+    (* Nothing to do for other procedure *)
+     * unfold f3_r_phi in H.
+       rewrite E1 in H.
+       rewrite E2 in H.
+       simpl in H.
+       unfold empty_r_precondition in H.
+       contradiction.
+(* Proof obligation for main relational property *)
 (* Verification of auxilliary proof obligation *)
-+ simpl. unfold f2_r_phi. simpl.
-  rewrite Bool.andb_false_r.
-  rewrite Proc.eqb_refl.
++ apply Vcg_Opt.Tc'_list.tc'_list_same.
   simpl.
-  auto.
-+ simpl. unfold f2_r_phi. simpl.
-  rewrite Bool.andb_false_r.
-  rewrite Proc.eqb_refl.
+  destruct n.
+  ++ unfold Vcg_Opt.Tc'_list.continuation.
+     simpl.
+     intros.
+     unfold f3_r_phi.
+     simpl.
+     rewrite Proc.eqb_refl.
+     simpl.
+     auto.
+  ++ destruct n; [auto | auto].
++ apply Vcg_Opt.Tc'_list.tc'_list_same.
   simpl.
-  auto.
+  destruct n.
+  ++ unfold Vcg_Opt.Tc'_list.continuation.
+     simpl.
+     intros.
+     unfold f3_r_phi.
+     simpl.
+     rewrite Proc.eqb_refl.
+     simpl.
+     auto.
+  ++ destruct n; [auto | auto].
 (* Main proof obligation *)
 + simpl.
   intros.
-  specialize (Hr (f2 :: f2 :: [])).
-  unfold f2_r_phi in Hr.
-  replace (list_beq Proc.t Proc.eqb [f2; f2] [f2; f2]) with true in Hr.
-  - specialize (Hr (s :: s0 :: []) (m' :: m'0 :: [])).
+  decompose [and] H0;clear H0.
+  decompose [and] H1;clear H1.
+  destruct (s X2) eqn:Horig.
+  * unfold f3_r_phi in H9.
+    simpl in H9. 
+    rewrite Proc.eqb_refl in H9.
+    simpl in H9.
+    unfold f3_r_phi in H5.
+    simpl in H5. 
+    rewrite Proc.eqb_refl in H5.
+    simpl in H5.
+    rewrite <- H9.
+    rewrite <- H5.
+    rewrite H4.
+    mem_s m'' X3 X3 0.
+    rewrite H8.
+    mem_s m''1 X3 X3 0.
+    reflexivity.
+    - rewrite H4.
+      mem_d m'' X3 X1 0.
+      mem_d m'' X3 X2 0.
+      rewrite H2.
+      mem_s s X1 X1 1.
+      mem_d s X1 X2 1.
+      lia.
+    - rewrite H8.
+      mem_d m''1 X3 X1 0.
+      mem_d m''1 X3 X2 0.
+      rewrite H0.
+      mem_s s0 X1 X1 0.
+      mem_d s0 X1 X2 0.
+      lia.
+ * specialize (Hr [f3; f3]).
+   unfold f3_r_phi in Hr.
+   rewrite internal_list_dec_lb in Hr; [ | apply Proc.eqb_eq | reflexivity].
+  - specialize (Hr [m''0; m''2] [m'; m'0]).
     simpl in Hr.
     apply Hr.
-    all: try Lia.lia.
-    split. apply H0.
-    split. apply H1.
+    all: try lia.
+    split. apply H7.
+    split. apply H11.
     auto.
-  - simpl.
-    symmetry.
-    eapply Bool.andb_true_iff.
-    split.
-    apply Proc.eqb_eq. reflexivity.
-    eapply Bool.andb_true_iff.
-    split.
-    apply Proc.eqb_eq. reflexivity.
-    auto.
+    rewrite H8.
+    mem_d m''1 X3 X1 0.
+    mem_d m''1 X3 X2 0.
+    mem_s m''1 X3 X3 0.
+    rewrite H0.
+    mem_s s0 X1 X1 0.
+    mem_d s0 X1 X2 0.
+    rewrite H4.
+    mem_d m'' X3 X1 0.
+    mem_d m'' X3 X2 0.
+    mem_s m'' X3 X3 0.
+    rewrite H2.
+    mem_s s X1 X1 1.
+    mem_d s X1 X2 1.
+    lia.
  Qed.
